[mlsexp] Add fromString + Rename parse to b_inputSexp

basis/SexpProgScript.sml
@@ -35,36 +35,62 @@ Quote add_cakeml:
   | Expr ses => PrettyPrinter.app_block "Expr" [PrettyPrinter.pp_list pp_sexp ses]
 End
 
+(* We will define two functions to generate s-expressions:
+   1. fromString, which is
+       - simple,
+       - fails with None (in the style of the SML basis)
+       - translated from mlsexp.
+   2. b_inputSexp, which is
+       - efficient (buffered input),
+       - fails with exceptions,
+       - written in CakeML, proved equivalent to definitions in mlsexp using
+         characteristic formulae (cf).
+
+   OPT If needed, fromString can be made more efficient by using mlstring
+     instead of a char list.
+ *)
+
 val _ = ml_prog_update open_local_block;
 
+(* Shared, but private, helpers and types *)
 val _ = register_type “:mlsexp$token”;
+val r = translate mlsexpTheory.parse_aux_def;
 
+(* Private helpers for fromString *)
+val r = translate mlsexpTheory.read_string_aux_def;
+val r = translate mlsexpTheory.read_string_def;
+val r = translate $ SRULE [isSpace_def] mlsexpTheory.read_symbol_def;
+val r = translate $ SRULE [isSpace_def] mlsexpTheory.lex_aux_def;
+val r = translate mlsexpTheory.lex_def;
+val r = translate mlsexpTheory.parse_def;
+
+(* Private helpers for b_inputSexp *)
 Quote add_cakeml:
-  fun read_string_aux input acc =
+  fun read_string_aux_imp input acc =
     case TextIO.b_input1 input of
       None => raise Fail "read_string_aux: unterminated string literal"
     | Some c =>
         if c = #"\"" then String.implode (List.rev acc) else
         if c = #"\\" then
           (case TextIO.b_input1 input of
-             None => read_string_aux input acc (* causes error: unterminated string *)
+             None => read_string_aux_imp input acc (* causes error: unterminated string *)
            | Some e =>
-               (if e = #"\\" then read_string_aux input (#"\""::acc) else
-                if e = #"0"  then read_string_aux input (#"\000"::acc) else
-                if e = #"n"  then read_string_aux input (#"\n"::acc) else
-                if e = #"r"  then read_string_aux input (#"\""::acc) else
-                if e = #"t"  then read_string_aux input (#"\""::acc) else
+               (if e = #"\\" then read_string_aux_imp input (#"\""::acc) else
+                if e = #"0"  then read_string_aux_imp input (#"\000"::acc) else
+                if e = #"n"  then read_string_aux_imp input (#"\n"::acc) else
+                if e = #"r"  then read_string_aux_imp input (#"\""::acc) else
+                if e = #"t"  then read_string_aux_imp input (#"\""::acc) else
                   raise Fail "read_string_aux: unrecognised escape"))
         else
-          read_string_aux input (c::acc)
+          read_string_aux_imp input (c::acc)
 End
 
 Quote add_cakeml:
-  fun read_string input = read_string_aux input []
+  fun read_string_imp input = read_string_aux_imp input []
 End
 
 Quote add_cakeml:
-  fun read_symbol input acc =
+  fun read_symbol_imp input acc =
     case TextIO.b_peekChar input of
       None => String.implode (List.rev acc)
     | Some c =>
@@ -72,42 +98,47 @@ Quote add_cakeml:
         then String.implode (List.rev acc)
         else (
           TextIO.b_input1 input;  (* Consume c *)
-          read_symbol input (c::acc))
+          read_symbol_imp input (c::acc))
 End
 
 Quote add_cakeml:
-  fun lex_aux depth input acc =
+  fun lex_aux_imp depth input acc =
     case TextIO.b_input1 input of
       None => if depth = 0 then acc
               else raise Fail "lex_aux: missing closing parenthesis"
     | Some c =>
-        if Char.isSpace c then lex_aux depth input acc
-        else if c = #"(" then lex_aux (depth + 1) input (Open::acc)
+        if Char.isSpace c then lex_aux_imp depth input acc
+        else if c = #"(" then lex_aux_imp (depth + 1) input (Open::acc)
         else if c = #")" then
           (if depth = 0 then raise Fail "lex_aux: too many closing parenthesis"
            else if depth = 1 then Close::acc
-           else lex_aux (depth - 1) input (Close::acc))
+           else lex_aux_imp (depth - 1) input (Close::acc))
         else if c = #"\"" then
-          let val s = read_string input in
+          let val s = read_string_imp input in
             if depth = 0 then [Symbol s]
-            else lex_aux depth input ((Symbol s)::acc) end
+            else lex_aux_imp depth input ((Symbol s)::acc) end
         else
-          let val s = read_symbol input [c] in
+          let val s = read_symbol_imp input [c] in
             if depth = 0 then [Symbol s]
-            else lex_aux depth input ((Symbol s)::acc) end
+            else lex_aux_imp depth input ((Symbol s)::acc) end
 End
 
 Quote add_cakeml:
-  fun lex input = lex_aux 0 input []
+  fun lex_imp input = lex_aux_imp 0 input []
 End
-
-val r = translate mlsexpTheory.parse_aux_def;
 
 val _ = ml_prog_update open_local_in_block;
 
+(* Exported functions *)
+val _ = next_ml_names := ["fromString"];
+val r = translate mlsexpTheory.fromString_def;
+
+(* If we were 100% consistent, we should call this parse_imp. Since it isn't a
+   neat name, and parse is already taken by the translated pure version, we
+   use b_inputSexp. *)
 Quote add_cakeml:
-  fun parse input =
-    case parse_aux (lex input) [] [] of
+  fun b_inputSexp input =
+    case parse_aux (lex_imp input) [] [] of
       [] => raise Fail "parse: empty input"
     | (v::_) => v
 End
@@ -121,8 +152,8 @@ val _ = ml_prog_update (close_module NONE);
 
 val st = get_ml_prog_state ();
 
-Definition read_string_aux_post_def:
-  read_string_aux_post s acc fs is fd =
+Definition read_string_aux_imp_post_def:
+  read_string_aux_imp_post s acc fs is fd =
     (case read_string_aux s acc of
      | INL (msg, rest) =>
          POSTe exn. SEP_EXISTS k.
@@ -135,10 +166,10 @@ Definition read_string_aux_post_def:
            &(STRING_TYPE slit slitv))
 End
 
-(* Can be used in read_string_aux_spec to finish proofs about base cases.
+(* Can be used in read_string_aux_imp_spec to finish proofs about base cases.
  * k indicates how much we moved forward (passed to forwardFD) *)
-fun read_string_aux_base_tac k =
-  (simp [read_string_aux_post_def, read_string_aux_def] \\ xsimpl
+fun read_string_aux_imp_base_tac k =
+  (simp [read_string_aux_imp_post_def, read_string_aux_def] \\ xsimpl
    \\ qexists k \\ xsimpl \\ simp [Fail_exn_def]);
 
 (* Useful when finishing up recursive cases. Takes care of instantiating k in
@@ -149,17 +180,17 @@ val STDIO_forwardFD_INSTREAM_STR_tac =
    \\ qmatch_goalsub_abbrev_tac ‘forwardFD fs fd kpx’
    \\ qexists ‘kpx’ \\ xsimpl);
 
-Theorem read_string_aux_spec[local]:
+Theorem read_string_aux_imp_spec[local]:
   ∀s acc accv p is fs fd.
     LIST_TYPE CHAR acc accv ⇒
-    app (p:'ffi ffi_proj) Sexp_read_string_aux_v [is; accv]
+    app (p:'ffi ffi_proj) Sexp_read_string_aux_imp_v [is; accv]
       (STDIO fs * INSTREAM_STR fd is s fs)
-      (read_string_aux_post s acc fs is fd)
+      (read_string_aux_imp_post s acc fs is fd)
 Proof
   ho_match_mp_tac read_string_aux_ind
   \\ rpt strip_tac
-  \\ qmatch_goalsub_abbrev_tac ‘read_string_aux_post s₁’
-  \\ xcf_with_def $ definition "Sexp_read_string_aux_v_def"
+  \\ qmatch_goalsub_abbrev_tac ‘read_string_aux_imp_post s₁’
+  \\ xcf_with_def $ definition "Sexp_read_string_aux_imp_v_def"
   (* [] *)
   >-
    (xlet ‘POSTv chv. SEP_EXISTS k.
@@ -169,7 +200,7 @@ Proof
     >- (xapp_spec b_input1_spec_str)
     \\ unabbrev_all_tac \\ gvs [OPTION_TYPE_def]
     \\ xmatch \\ xlet_autop \\ xraise
-    \\ read_string_aux_base_tac ‘k’)
+    \\ read_string_aux_imp_base_tac ‘k’)
   (* c::rest *)
   >-
    (xlet ‘POSTv chv. SEP_EXISTS k.
@@ -185,11 +216,11 @@ Proof
       \\ xapp \\ xsimpl
       \\ first_assum $ irule_at (Pos hd)
       \\ rpt strip_tac
-      \\ read_string_aux_base_tac ‘k’)
+      \\ read_string_aux_imp_base_tac ‘k’)
     \\ xlet_autop
     \\ xif (* c = \ *)
     >-
-     (rename [‘read_string_aux_post (STRING _ s)’]
+     (rename [‘read_string_aux_imp_post (STRING _ s)’]
       \\ xlet ‘POSTv chv. SEP_EXISTS k₁.
                  STDIO (forwardFD fs fd (k + k₁)) *
                  INSTREAM_STR fd is (TL s) (forwardFD fs fd (k + k₁)) *
@@ -203,7 +234,7 @@ Proof
        (xmatch \\ xapp
         \\ first_assum $ irule_at (Pos hd)
         \\ qexistsl [‘forwardFD fs fd (k + k₁)’, ‘fd’, ‘emp’]
-        \\ simp [read_string_aux_post_def, read_string_aux_def]
+        \\ simp [read_string_aux_imp_post_def, read_string_aux_def]
         \\ STDIO_forwardFD_INSTREAM_STR_tac)
       \\ xmatch
       (* escape characters *)
@@ -216,25 +247,25 @@ Proof
           \\ xapp
           \\ simp [LIST_TYPE_def]
           \\ qexistsl [‘emp’, ‘forwardFD fs fd (k + k₁)’, ‘fd’]
-          \\ simp [read_string_aux_post_def, read_string_aux_def]
+          \\ simp [read_string_aux_imp_post_def, read_string_aux_def]
           \\ ntac 2 CASE_TAC
           \\ STDIO_forwardFD_INSTREAM_STR_tac))
       (* unrecognised escape *)
       \\ xlet_autop \\ xraise
-      \\ read_string_aux_base_tac ‘k + k₁’)
+      \\ read_string_aux_imp_base_tac ‘k + k₁’)
   (* simply push c and recurse *)
   \\ xlet_autop
   \\ gvs []
   \\ xapp
   \\ simp [LIST_TYPE_def]
   \\ qexistsl [‘emp’, ‘forwardFD fs fd k’, ‘fd’]
-  \\ simp [read_string_aux_post_def, read_string_aux_def]
+  \\ simp [read_string_aux_imp_post_def, read_string_aux_def]
   \\ ntac 2 CASE_TAC
   \\ STDIO_forwardFD_INSTREAM_STR_tac)
 QED
 
-Theorem read_string_spec:
-  app (p:'ffi ffi_proj) Sexp_read_string_v [is]
+Theorem read_string_imp_spec:
+  app (p:'ffi ffi_proj) Sexp_read_string_imp_v [is]
     (STDIO fs * INSTREAM_STR fd is s fs)
     (case read_string s of
      | INL (msg, rest) =>
@@ -247,17 +278,17 @@ Theorem read_string_spec:
            INSTREAM_STR fd is rest (forwardFD fs fd k) *
            &(STRING_TYPE slit slitv))
 Proof
-  xcf_with_def $ definition "Sexp_read_string_v_def"
+  xcf_with_def $ definition "Sexp_read_string_imp_v_def"
   \\ xlet_autop \\ xapp
-  \\ simp [read_string_aux_post_def, read_string_def]
+  \\ simp [read_string_aux_imp_post_def, read_string_def]
   \\ qexistsl [‘emp’, ‘s’, ‘fs’, ‘fd’, ‘[]’]
   \\ simp [LIST_TYPE_def] \\ xsimpl
 QED
 
-Theorem read_symbol_spec[local]:
+Theorem read_symbol_imp_spec[local]:
   ∀s acc accv p is fs fd.
     LIST_TYPE CHAR acc accv ⇒
-    app (p:'ffi ffi_proj) Sexp_read_symbol_v [is; accv]
+    app (p:'ffi ffi_proj) Sexp_read_symbol_imp_v [is; accv]
       (STDIO fs * INSTREAM_STR fd is s fs)
       (case read_symbol s acc of
        | (slit, rest) =>
@@ -269,7 +300,7 @@ Proof
   Induct
   \\ rpt strip_tac
   \\ qmatch_goalsub_abbrev_tac ‘read_symbol s₁’
-  \\ xcf_with_def $ definition "Sexp_read_symbol_v_def"
+  \\ xcf_with_def $ definition "Sexp_read_symbol_imp_v_def"
   >- (* [] *)
    (xlet ‘POSTv chv. SEP_EXISTS k.
             STDIO (forwardFD fs fd k) *
@@ -325,8 +356,8 @@ Proof
     \\ STDIO_forwardFD_INSTREAM_STR_tac)
 QED
 
-Definition lex_aux_post_def:
-  lex_aux_post depth s acc fs is fd =
+Definition lex_aux_imp_post_def:
+  lex_aux_imp_post depth s acc fs is fd =
     (case lex_aux depth s acc of
      | INL (msg, rest) =>
          POSTe exn. SEP_EXISTS k.
@@ -341,23 +372,23 @@ End
 
 val MLSEXP_TOKEN_TYPE_def = theorem "MLSEXP_TOKEN_TYPE_def";
 
-(* Analogous to read_string_aux_base_tac *)
-fun lex_aux_base_tac k =
-  (simp [lex_aux_post_def, lex_aux_def] \\ xsimpl
+(* Analogous to read_string_aux_imp_base_tac *)
+fun lex_aux_imp_base_tac k =
+  (simp [lex_aux_imp_post_def, lex_aux_def] \\ xsimpl
    \\ qexists k \\ xsimpl
    \\ simp [LIST_TYPE_def, MLSEXP_TOKEN_TYPE_def, Fail_exn_def]);
 
-Theorem lex_aux_spec:
+Theorem lex_aux_imp_spec:
   ∀ depth s acc depthv accv p is fs fd.
     NUM depth depthv ∧ LIST_TYPE MLSEXP_TOKEN_TYPE acc accv ⇒
-    app (p:'ffi ffi_proj) Sexp_lex_aux_v [depthv; is; accv]
+    app (p:'ffi ffi_proj) Sexp_lex_aux_imp_v [depthv; is; accv]
       (STDIO fs * INSTREAM_STR fd is s fs)
-      (lex_aux_post depth s acc fs is fd)
+      (lex_aux_imp_post depth s acc fs is fd)
 Proof
   ho_match_mp_tac lex_aux_ind
   \\ rpt strip_tac
-  \\ qmatch_goalsub_abbrev_tac ‘lex_aux_post _ s₁’
-  \\ xcf_with_def $ definition "Sexp_lex_aux_v_def"
+  \\ qmatch_goalsub_abbrev_tac ‘lex_aux_imp_post _ s₁’
+  \\ xcf_with_def $ definition "Sexp_lex_aux_imp_v_def"
   (* [] *)
   >-
    (xlet ‘POSTv chv. SEP_EXISTS k.
@@ -368,9 +399,9 @@ Proof
     \\ unabbrev_all_tac \\ gvs [OPTION_TYPE_def]
     \\ xmatch \\ xlet_autop
     \\ xif
-    >- (xvar \\ lex_aux_base_tac ‘k’)
+    >- (xvar \\ lex_aux_imp_base_tac ‘k’)
     \\ xlet_autop
-    \\ xraise \\ lex_aux_base_tac ‘k’)
+    \\ xraise \\ lex_aux_imp_base_tac ‘k’)
   (* c::cs *)
   \\ xlet ‘POSTv chv. SEP_EXISTS k.
             STDIO (forwardFD fs fd k) *
@@ -378,14 +409,14 @@ Proof
             &OPTION_TYPE CHAR (oHD s₁) chv’
   >- (xapp_spec b_input1_spec_str)
   \\ unabbrev_all_tac \\ gvs [OPTION_TYPE_def]
-  \\ rename [‘lex_aux_post _ (STRING c s)’]
+  \\ rename [‘lex_aux_imp_post _ (STRING c s)’]
   \\ xmatch
   \\ xlet_autop
   \\ xif >-
    (last_x_assum $ drule_all_then assume_tac
     \\ xapp
     \\ qexistsl [‘emp’, ‘forwardFD fs fd k’, ‘fd’]
-    \\ simp [lex_aux_post_def, lex_aux_def]
+    \\ simp [lex_aux_imp_post_def, lex_aux_def]
     \\ ntac 2 CASE_TAC
     \\ STDIO_forwardFD_INSTREAM_STR_tac)
   \\ xlet_autop
@@ -393,26 +424,26 @@ Proof
    (ntac 3 xlet_autop
     \\ xapp
     \\ qexistsl [‘emp’, ‘forwardFD fs fd k’, ‘fd’]
-    \\ gvs [lex_aux_post_def, lex_aux_def]
+    \\ gvs [lex_aux_imp_post_def, lex_aux_def]
     \\ conj_tac >- (simp [LIST_TYPE_def, MLSEXP_TOKEN_TYPE_def])
     \\ ntac 2 CASE_TAC
     \\ STDIO_forwardFD_INSTREAM_STR_tac)
   \\ xlet_autop
   \\ xif >-
    (xlet_autop
-    \\ xif >- (xlet_autop \\ xraise \\ lex_aux_base_tac ‘k’)
+    \\ xif >- (xlet_autop \\ xraise \\ lex_aux_imp_base_tac ‘k’)
     \\ xlet_autop
-    \\ xif >- (xlet_autop \\ xcon \\ lex_aux_base_tac ‘k’)
+    \\ xif >- (xlet_autop \\ xcon \\ lex_aux_imp_base_tac ‘k’)
     \\ ntac 3 xlet_autop
     \\ xapp
     \\ qexistsl [‘emp’, ‘forwardFD fs fd k’, ‘fd’]
-    \\ gvs [lex_aux_post_def, lex_aux_def]
+    \\ gvs [lex_aux_imp_post_def, lex_aux_def]
     \\ conj_tac >- (simp [LIST_TYPE_def, MLSEXP_TOKEN_TYPE_def])
     \\ ntac 2 CASE_TAC
     \\ STDIO_forwardFD_INSTREAM_STR_tac)
   \\ xlet_autop
   \\ xif >-
-   (simp [lex_aux_post_def, lex_aux_def, isSpace_def]
+   (simp [lex_aux_imp_post_def, lex_aux_def, isSpace_def]
     \\ namedCases_on ‘mlsexp$read_string s’ ["l", "r"]
     >-
      (namedCases_on ‘l’ ["msg rest"]
@@ -440,13 +471,13 @@ Proof
     >-
      (ntac 2 xlet_autop \\ xcon
       \\ simp [LIST_TYPE_def, MLSEXP_TOKEN_TYPE_def]
-      \\ lex_aux_base_tac ‘k’)
+      \\ lex_aux_imp_base_tac ‘k’)
     \\ ntac 2 xlet_autop \\ xapp
     \\ qexistsl [‘emp’, ‘forwardFD fs fd k’, ‘fd’]
-    \\ simp [LIST_TYPE_def, MLSEXP_TOKEN_TYPE_def, lex_aux_post_def]
+    \\ simp [LIST_TYPE_def, MLSEXP_TOKEN_TYPE_def, lex_aux_imp_post_def]
     \\ ntac 2 CASE_TAC
     \\ STDIO_forwardFD_INSTREAM_STR_tac)
-  \\ simp [lex_aux_post_def, lex_aux_def]
+  \\ simp [lex_aux_imp_post_def, lex_aux_def]
   \\ ntac 2 xlet_autop
   \\ namedCases_on ‘read_symbol s [c]’ ["sym rest"]
   \\ xlet ‘POSTv symv. SEP_EXISTS k.
@@ -459,16 +490,16 @@ Proof
     \\ simp [LIST_TYPE_def]
     \\ STDIO_forwardFD_INSTREAM_STR_tac)
   \\ xlet_autop
-  \\ xif >- (ntac 2 xlet_autop \\ xcon \\ lex_aux_base_tac ‘k’)
+  \\ xif >- (ntac 2 xlet_autop \\ xcon \\ lex_aux_imp_base_tac ‘k’)
   \\ ntac 2 xlet_autop \\ xapp
   \\ qexistsl [‘emp’, ‘forwardFD fs fd k’, ‘fd’]
-  \\ simp [LIST_TYPE_def, MLSEXP_TOKEN_TYPE_def, lex_aux_post_def]
+  \\ simp [LIST_TYPE_def, MLSEXP_TOKEN_TYPE_def, lex_aux_imp_post_def]
   \\ ntac 2 CASE_TAC
   \\ STDIO_forwardFD_INSTREAM_STR_tac
 QED
 
-Theorem lex_spec:
-  app (p:'ffi ffi_proj) Sexp_lex_v [is]
+Theorem lex_imp_spec:
+  app (p:'ffi ffi_proj) Sexp_lex_imp_v [is]
     (STDIO fs * INSTREAM_STR fd is s fs)
     (case lex s of
      | INL (msg, rest) =>
@@ -481,15 +512,15 @@ Theorem lex_spec:
          INSTREAM_STR fd is rest (forwardFD fs fd k) *
          &(LIST_TYPE MLSEXP_TOKEN_TYPE toks tokvs))
 Proof
-  xcf_with_def $ definition "Sexp_lex_v_def"
+  xcf_with_def $ definition "Sexp_lex_imp_v_def"
   \\ xlet_autop \\ xapp
-  \\ simp [lex_aux_post_def, lex_def]
+  \\ simp [lex_aux_imp_post_def, lex_def]
   \\ qexistsl [‘emp’, ‘s’, ‘fs’, ‘fd’, ‘[]’]
   \\ simp [LIST_TYPE_def, MLSEXP_TOKEN_TYPE_def] \\ xsimpl
 QED
 
-Theorem parse_spec:
-  app (p:'ffi ffi_proj) Sexp_parse_v [is]
+Theorem b_inputSexp_spec:
+  app (p:'ffi ffi_proj) Sexp_b_inputSexp_v [is]
     (STDIO fs * INSTREAM_STR fd is s fs)
     (case parse s of
      | INL (msg, rest) =>
@@ -502,7 +533,7 @@ Theorem parse_spec:
          INSTREAM_STR fd is rest (forwardFD fs fd k) *
          &(SEXP_TYPE se sev))
 Proof
-  xcf_with_def $ definition "Sexp_parse_v_def"
+  xcf_with_def $ definition "Sexp_b_inputSexp_v_def"
   \\ ntac 2 xlet_autop
   \\ simp [parse_def]
   \\ namedCases_on ‘lex s’ ["l", "r"]
